concurrency/juicy/semax_conc_pred.v
@@ -1,159 +1,29 @@
-Require Import VST.msl.msl_standard.
-Require Import VST.msl.seplog.
-Require Import VST.veric.base.
-Require Import VST.veric.compcert_rmaps.
-Require Import VST.veric.juicy_mem.
-Require Import VST.veric.juicy_mem_lemmas.
-Require Import VST.veric.juicy_mem_ops.
-Require Import VST.veric.juicy_extspec.
-Require Import VST.veric.tycontext.
-Require Import VST.veric.expr2.
-Require Import VST.veric.semax.
-Require Import VST.veric.semax_call.
-Require Import VST.veric.semax_ext.
-Require Import VST.veric.semax_ext_oracle.
-Require Import VST.veric.juicy_safety.
-Require Import VST.veric.Clight_core.
-Require Import VST.veric.res_predicates.
 Require Import VST.veric.SeparationLogic.
-Require Import VST.sepcomp.extspec.
-Require Import VST.floyd.reptype_lemmas.
-Require Import VST.floyd.field_at.
-Require Import VST.floyd.nested_field_lemmas.
-Require Import VST.floyd.client_lemmas.
-Require Import VST.floyd.jmeq_lemmas.
 Require Import VST.concurrency.common.lksize.
-Require Import VST.concurrency.conclib.
+
+Section mpred.
+
+Context `{!heapGS Σ}.
 
 Definition lock_inv : share -> val -> mpred -> mpred :=
   fun sh v R =>
-    (EX b : block, EX ofs : _,
-      !!(v = Vptr b ofs) &&
-      LKspec LKSIZE
-        R sh (b, Ptrofs.unsigned ofs))%logic.
+    (∃ b : block, ∃ ofs : _,
+      ⌜v = Vptr b ofs⌝ ∧
+      LKspec LKSIZE R sh (b, Ptrofs.unsigned ofs)).
 
-Definition rec_inv sh v (Q R: mpred): Prop :=
-  (R = Q * |>lock_inv sh v R)%logic.
+(*Definition rec_inv sh v (Q R: mpred): Prop :=
+  (R = Q * |>lock_inv sh v R).
 
 Definition weak_rec_inv sh v (Q R: mpred): mpred :=
-  (! (R <=> Q * |>lock_inv sh v R))%pred.
+  (! (R <=> Q * |>lock_inv sh v R))%pred.*)
 
-Lemma lockinv_isptr sh v R : lock_inv sh v R = (!! isptr v && lock_inv sh v R)%logic.
+Lemma lockinv_isptr sh v R : lock_inv sh v R ⊣⊢ (⌜isptr v⌝ ∧ lock_inv sh v R).
 Proof.
-  assert (D : isptr v \/ ~isptr v) by (destruct v; simpl; auto).
-  destruct D.
-  - rewrite prop_true_andp; auto.
-  - rewrite prop_false_andp; auto.
-    apply pred_ext.
-    + unfold lock_inv. Transparent mpred. Intros b ofs. Opaque mpred. subst; simpl in *; tauto.
-    + apply FF_left.
+  rewrite comm; apply add_andp.
+  by iIntros "(% & % & -> & ?)".
 Qed.
 
-Lemma unfash_fash_equiv: forall P Q: mpred,
-  (P <=> Q |--
-  (subtypes.unfash (subtypes.fash P): mpred) <=> (subtypes.unfash (subtypes.fash Q): mpred))%pred.
-Proof.
-  intros.
-  constructor; apply eqp_unfash.
-  rewrite eqp_nat.
-  apply predicates_hered.andp_right; eapply predicates_hered.derives_trans, subtypes.fash_K;
-    apply subtypes.fash_derives.
-  - apply predicates_hered.andp_left1; auto.
-  - apply predicates_hered.andp_left2; auto.
-Qed.
-
-Lemma iffp_equiv: forall P1 Q1 P2 Q2: mpred,
-  ((P1 <=> Q1) && (P2 <=> Q2) |-- (P1 <--> P2) <=> (Q1 <--> Q2))%pred.
-Proof.
-  intros.
-  constructor; apply eqp_andp; apply subp_eqp; apply subtypes.subp_imp.
-  - apply predicates_hered.andp_left1.
-    rewrite eqp_comm; apply eqp_subp.
-  - apply predicates_hered.andp_left2.
-    apply eqp_subp.
-  - apply predicates_hered.andp_left1.
-    apply eqp_subp.
-  - apply predicates_hered.andp_left2.
-    rewrite eqp_comm; apply eqp_subp.
-  - apply predicates_hered.andp_left2.
-    rewrite eqp_comm; apply eqp_subp.
-  - apply predicates_hered.andp_left1.
-    apply eqp_subp.
-  - apply predicates_hered.andp_left2.
-    apply eqp_subp.
-  - apply predicates_hered.andp_left1.
-    rewrite eqp_comm; apply eqp_subp.
-Qed.
-
-Lemma sepcon_equiv: forall P1 Q1 P2 Q2: mpred,
-  ((P1 <=> Q1) && (P2 <=> Q2) |-- (P1 * P2) <=> (Q1 * Q2))%pred.
-Proof.
-  intros.
-  constructor; apply eqp_sepcon.
-  - apply predicates_hered.andp_left1; auto.
-  - apply predicates_hered.andp_left2; auto.
-Qed.
-
-Lemma later_equiv: forall P Q: mpred,
-  (P <=> Q |-- |> P <=> |> Q)%pred.
-Proof.
-  intros.
-  constructor; eapply predicates_hered.derives_trans, subtypes.eqp_later1.
-  apply predicates_hered.now_later.
-Qed.
-
-Lemma nonexpansive_lock_inv : forall sh p, nonexpansive (lock_inv sh p).
-Proof.
-  intros.
-  unfold lock_inv.
-  apply @exists_nonexpansive.
-  intros b.
-  apply @exists_nonexpansive.
-  intros y.
-  apply @conj_nonexpansive.
-  apply @const_nonexpansive.
-
-  unfold LKspec.
-  apply forall_nonexpansive; intros.
-  hnf; intros.
-  intros n ?.
-  assert (forall y: rmap, (n >= level y)%nat -> (app_pred P y <-> app_pred Q y)).
-  {
-    clear - H.
-    intros; specialize (H y H0).
-    destruct H.
-    split; [eapply H | eapply H1]; eauto.
-  }
-  simpl; split; intros.
-  + if_tac; auto.
-    destruct H4 as [p0 ?].
-    exists p0.
-    rewrite H4; f_equal.
-    f_equal.
-    extensionality ts; clear ts.
-    clear H4 H5 p0.
-    apply ext_level in H3.
-    apply predicates_hered.pred_ext; hnf; intros ? [? ?]; split; auto.
-    - apply necR_level in H2.
-      rewrite <- H0 by lia; auto.
-    - apply necR_level in H2.
-      rewrite H0 by lia; auto.
-  + if_tac; auto.
-    destruct H4 as [p0 ?].
-    exists p0.
-    rewrite H4; f_equal.
-    f_equal.
-    extensionality ts; clear ts.
-    clear H4 H5 p0.
-    apply ext_level in H3.
-    apply predicates_hered.pred_ext; hnf; intros ? [? ?]; split; auto.
-    - apply necR_level in H2.
-      rewrite H0 by lia; auto.
-    - apply necR_level in H2.
-      rewrite <- H0 by lia; auto.
-Qed.
-
-Lemma rec_inv1_nonexpansive: forall sh v Q,
+(*Lemma rec_inv1_nonexpansive: forall sh v Q,
   nonexpansive (weak_rec_inv sh v Q).
 Proof.
   intros.
@@ -204,4 +74,6 @@ Proof.
   intros.
   rewrite H at 1 4.
   split; intros; hnf; intros; auto.
-Qed.
+Qed.*)
+
+End mpred.
