concurrency/common/ClightSemanticsForMachines.v
@@ -8,8 +8,6 @@
 *)
 
 Require Import compcert.common.Memory.
-Require Import VST.veric.compcert_rmaps.
-Require Import VST.veric.juicy_mem.
 Require Import VST.veric.res_predicates.
 
 (*IM using proof irrelevance!*)
