floyd/client_lemmas.v
@@ -1,8 +1,6 @@
 Require Import VST.floyd.base2.
 Require Export VST.floyd.canon.
 Import LiftNotation.
-Import compcert.lib.Maps.
-Local Open Scope logic.
 
 Lemma SEP_entail:
  forall R' Delta P Q R,
